replissSem1.thy
@@ -1,6 +1,7 @@
 theory replissSem1
 imports Main
   "~~/src/HOL/Library/Multiset"
+  "~~/src/HOL/Library/Option_ord"
   "~/work/afp/thys/Proof_Strategy_Language/PSL" 
 begin
 
@@ -47,6 +48,21 @@ typedecl procedureName
 type_synonym procedureImpl = "localState \<Rightarrow> localAction"
 
 datatype transactionStatus = Uncommited | Commited 
+
+instantiation transactionStatus :: linorder 
+begin
+definition "less_eq_transactionStatus x y \<equiv> x = Uncommited \<or> y = Commited"
+definition "less_transactionStatus x y \<equiv> x = Uncommited \<and> y = Commited"
+instance 
+apply standard
+using transactionStatus.exhaust by (auto simp add: less_eq_transactionStatus_def less_transactionStatus_def )
+end  
+
+lemmas transactionStatus_less_simps[simp] = less_eq_transactionStatus_def less_transactionStatus_def
+
+lemma onlyCommitedGreater: "a \<triangleq> Commited" if "a\<ge>Some Commited" for a
+  by (smt dual_order.antisym dual_order.trans less_eq_option_None_is_None less_eq_option_Some less_eq_transactionStatus_def order_refl split_option_ex that)
+          
 
 record operationContext = 
   calls :: "callId \<rightharpoonup> call"
@@ -645,180 +661,5 @@ proof -
 qed  
 
 
-definition state_wellFormed :: "state \<Rightarrow> bool" where
-"state_wellFormed state \<equiv> \<exists>tr. initialState (prog state) ~~ tr \<leadsto>* state"
-
-lemma state_wellFormed_init[simp]:
-"state_wellFormed (initialState program)"
-  by (metis distributed_state.select_convs(1) initialState_def state_wellFormed_def steps_refl)
-
-lemma steps_do_not_change_prog: 
-assumes "S ~~ tr \<leadsto>* S'"
-shows "prog S' = prog S"
-using assms proof (induct rule: steps.induct)
-  case (steps_refl S)
-  then show ?case by simp
-next
-  case (steps_step S tr S' a S'')
-  hence [simp]: "prog S' = prog S" by simp
-  from `S' ~~ a \<leadsto> S''`
-  show ?case 
-    apply (rule step.cases)
-    apply auto
-    done
-qed
-  
-lemma state_wellFormed_combine:
-assumes wf: "state_wellFormed S"
-and steps: "S ~~ tr \<leadsto>* S'"
-shows "state_wellFormed S'"
-proof -
-  from steps 
-  have "prog S' = prog S"
-    using steps_do_not_change_prog by auto
-
- from wf obtain tr1 where "initialState (prog S) ~~ tr1 \<leadsto>* S"
-   using state_wellFormed_def by blast 
- with steps
- have "initialState (prog S) ~~ tr1@tr \<leadsto>* S'"
-   using steps_append by blast
- with `prog S' = prog S`
- have "initialState (prog S') ~~ tr1@tr \<leadsto>* S'" by simp
- thus "state_wellFormed S'"
-  using state_wellFormed_def by auto 
-qed  
-
-lemma step_prog_invariant:
-"S ~~ tr \<leadsto>* S' \<Longrightarrow> prog S' = prog S"
-apply (induct rule: steps.induct)
-apply auto
-apply (erule step.cases)
-apply auto
-done
-
-thm full_nat_induct
-
-
-lemma steps_induct[consumes 1, case_names initial step[steps IH step]]:
-assumes a1: "init ~~ tr \<leadsto>*  S"
-    and a2: "P [] init"
-    and a3: "\<And>S' tr a S''. \<lbrakk>init ~~ tr \<leadsto>*  S'; P tr S'; S' ~~ a \<leadsto> S''\<rbrakk> \<Longrightarrow> P (tr@[a]) S''"
-shows "P tr S"
-proof -
-  have h: "\<lbrakk>S ~~ tr \<leadsto>* s; P [] init; S = init; 
-      \<And>S' tr a S''. \<lbrakk>init ~~ tr \<leadsto>*  S'; P tr S'; S' ~~ a \<leadsto> S''\<rbrakk> \<Longrightarrow> P (tr@[a]) S''\<rbrakk> \<Longrightarrow> P tr s" for S tr s
-    proof (induct rule: steps.induct)
-      case (steps_refl S)                        
-      then show ?case by simp
-    next
-      case (steps_step S tr S' a S'')
-      have "P tr S'"
-        apply (rule steps_step(2))
-        using initialState_def step_prog_invariant steps_step.hyps(1) steps_step.prems(1) steps_step.prems(2) apply auto[1]
-        using initialState_def step_prog_invariant steps_step.hyps(1) steps_step.prems(2) apply auto[1]
-        by (simp add: steps_step.prems(3))
-      show ?case
-      proof (rule a3)
-        show "init ~~ tr \<leadsto>* S'"
-          using steps_step.hyps(1) steps_step.prems(2) by auto
-        show "P tr S'" using `P tr S'` .
-        show "S' ~~ a \<leadsto> S''"
-          by (simp add: steps_step.hyps(3)) 
-      qed
-    qed
-  show ?thesis
-  using a1 a2
-  proof (rule h)
-    show "init = init" ..
-    show "\<And>S' tr a S''. \<lbrakk>init ~~ tr \<leadsto>* S'; P tr S'; S' ~~ a \<leadsto> S''\<rbrakk> \<Longrightarrow> P (tr @ [a]) S''"
-      using a3 by auto
-  qed  
-qed
-
-
-lemma steps_induct2[consumes 1, case_names initial step[steps IH step]]:
-assumes a1: "initialState progr ~~ tr \<leadsto>*  S"
-    and a2: "P [] (initialState progr)"
-    and a3: "\<And>S' tr a S''. \<lbrakk>initialState progr ~~ tr \<leadsto>*  S'; P tr S'; S' ~~ a \<leadsto> S''\<rbrakk> \<Longrightarrow> P (tr@[a]) S''"
-shows "P tr S"
-  using a1 a2 a3 steps_induct by blast
-
-
-lemma wellFormed_induct[consumes 1, case_names initial step]:
-"\<lbrakk>state_wellFormed s; P (initialState (prog s)); \<And>t a s. \<lbrakk>state_wellFormed t; P t; t ~~ a \<leadsto> s\<rbrakk> \<Longrightarrow> P s\<rbrakk> \<Longrightarrow> P s"
-apply (auto simp add: state_wellFormed_def)
-apply (erule(1) steps_induct)
-by (metis prod.collapse state_wellFormed_def state_wellFormed_init step_prog_invariant steps_append)
-
-
-
-lemma wellFormed_callOrigin_dom:
-assumes a1: "state_wellFormed S"
-shows "dom (callOrigin S) = dom (calls S)"
-using a1 apply (induct rule: wellFormed_induct)
-apply (simp add: initialState_def)
-apply (erule step.cases)
-apply (auto split: if_splits)
-  apply blast
-  by blast
-
-lemma wellFormed_callOrigin_dom2[simp]: 
-"\<lbrakk>calls S c = None; state_wellFormed S\<rbrakk> \<Longrightarrow>  callOrigin S c = None"
-  using wellFormed_callOrigin_dom by force
-
-
-lemma wellFormed_visibleCallsSubsetCalls_h:
-assumes a1: "state_wellFormed S"
-shows "happensBefore S \<subseteq> dom (calls S) \<times> dom (calls S)"
-   and "\<And>vis s. visibleCalls S s \<triangleq> vis \<Longrightarrow> state_wellFormed S \<Longrightarrow> vis \<subseteq> dom (calls S)" 
-using a1 apply (induct rule: wellFormed_induct)
-apply (simp add: initialState_def)
-apply (simp add: initialState_def)
-apply (erule step.cases)
-apply (auto split: if_splits)
-  apply blast
-  apply blast
-apply (erule step.cases)
-apply (auto split: if_splits)
-  apply blast
-  apply blast
-  apply blast
-  apply (auto simp add: callsInTransactionH_contains downwardsClosure_in split: option.splits)[1]
-  apply (metis not_None_eq wellFormed_callOrigin_dom2)
-  apply blast
-  apply blast
-  apply blast
-  apply blast
-  apply blast
-  apply blast
-  apply blast
-  apply blast
-done  
-  
-
-    
-lemma wellFormed_visibleCallsSubsetCalls:
-assumes a1: "state_wellFormed A"
-    and a2: "visibleCalls A s \<triangleq> vis"
-shows "vis \<subseteq> dom (calls A)"
-  using a1 a2 wellFormed_visibleCallsSubsetCalls_h(2) by auto
-
-lemma wellFormed_currentTransaction_unique_h:
-assumes a1: "state_wellFormed S"
-shows "\<forall>sa sb t. currentTransaction S sa \<triangleq> t \<longrightarrow> currentTransaction S sb \<triangleq> t \<longrightarrow>  sa = sb"
-  and "\<forall>sa t. currentTransaction S sa \<triangleq> t \<longrightarrow> transactionStatus S t \<triangleq> Uncommited"
-using a1 apply (induct  rule: wellFormed_induct)
-apply (simp add: initialState_def)
-apply (simp add: initialState_def)
-apply (erule step.cases)
-apply (auto split: if_splits)
-apply (erule step.cases)
-apply (auto split: if_splits)
-done   
-  
-lemmas wellFormed_currentTransaction_unique = wellFormed_currentTransaction_unique_h(1)[rule_format]
-lemmas wellFormed_currentTransactionUncommited[simp] = wellFormed_currentTransaction_unique_h(2)[rule_format]
-    
-  
   
 end
